Isabelle/Grammar.thy
@@ -119,7 +119,7 @@ by (simp add: norm_of_variables_def ns_distr)
 lemma nov_distr': "norm_of_variables gr (x # y) = norm_of_variables gr [x] + norm_of_variables gr y"
 by (rule nov_distr[of _ "[x]", simplified])
 
-lemma nov_singleton: "norm_of_variables gr [v] = fst (lookup (norms_of_grammar gr) v)"
+lemma nov_singleton: "norm_of_variables gr [v] = fst (lookup (norms_of_grammar_new gr) v)"
 by (simp add: norm_of_variables_def ns_singleton)
 
 lemma nov_nog:
@@ -135,6 +135,13 @@ lemma nov_nog':
       and "(v, rules) \<in> set gr"
     shows "norm_of_variables gr vs < norm_of_variables gr [v]" using assms
 by (auto simp add: nov_nog)
+
+lemma nov_nog_new':
+  assumes "gram_valid gr"
+      and "(t, vs) = snd (lookup (norms_of_grammar_new gr) v)"
+      and "(v, rules) \<in> set gr"
+    shows "norm_of_variables gr vs < norm_of_variables gr [v]" using assms
+sorry
 
 lemma nov_greater_zero: "gram_valid gr \<Longrightarrow> (v, rules) \<in> set gr \<Longrightarrow> 0 < norm_of_variables gr [v]"
 sorry
@@ -162,8 +169,26 @@ sorry
   norms_of_grammar_new
  *****************************************************************************)
 
-lemma nog_new_fst_is_gr_fst: "gram_normed gr \<Longrightarrow> map fst gr = map fst (norms_of_grammar_new gr)"
+(* lemma nog_new_fst_is_gr_fst: "gram_normed gr \<Longrightarrow> map fst gr = map fst (norms_of_grammar_new gr)"
+sorry *)
+
+lemma nog_new_mnor:
+  assumes "gram_valid gr"
+      and "(v, rules) \<in> set gr"
+    shows "lookup (norms_of_grammar_new gr) v = min_norm_of_rules (norms_of_grammar_new gr) rules" using assms
 sorry
+
+lemma nog_new_sufficient:
+  assumes "gram_valid gr"
+      and "(v, rules) \<in> set gr"
+    shows "norms_sufficient (norms_of_grammar_new gr) rules"
+sorry
+
+lemma nog_new_in_rules:
+  assumes "gram_valid gr"
+      and "(v, rules) \<in> set gr"
+    shows "snd (lookup (norms_of_grammar_new gr) v) \<in> set rules" using assms
+by (auto simp add: nog_new_mnor nog_new_sufficient mnor_in_rules)
 
 
 (*****************************************************************************
@@ -173,7 +198,7 @@ sorry
 termination minimal_word_of_variables
   apply (relation "measure (\<lambda>(gr, vs). norm_of_variables gr vs)", auto)
   apply (subst nov_distr')
-  apply (auto simp add: add_commute add_strict_increasing2 nov_nog')
+  apply (auto simp add: add_commute add_strict_increasing2 nov_nog_new')
   apply (subst nov_distr')
 by (auto simp add: nov_greater_zero)
 
@@ -187,13 +212,13 @@ lemma mwov_dist:
            minimal_word_of_variables gr v1 @ minimal_word_of_variables gr v2" using assms
 proof (induct v1 arbitrary: v2)
   case (Cons a v1)
-  then show ?case by (case_tac "snd (lookup (norms_of_grammar gr) a)") auto
+  then show ?case by (case_tac "snd (lookup (norms_of_grammar_new gr) a)") auto
 qed auto
 
 lemma mwov_len_calcs_nog:
   assumes "gram_valid gr"
       and "v \<in> keys gr"
-      and "(n, nt, nrt) = lookup (norms_of_grammar gr) v"
+      and "(n, nt, nrt) = lookup (norms_of_grammar_new gr) v"
     shows "Suc (length (minimal_word_of_variables gr nrt)) = n" using assms
 sorry
 
@@ -204,7 +229,7 @@ theorem mwov_len_calcs_nov:
 proof (induct gr v rule: mwov_induct)
   case (Cons_vars gr vh vt)
 
-  def nogh \<equiv> "lookup (norms_of_grammar gr) vh"
+  def nogh \<equiv> "lookup (norms_of_grammar_new gr) vh"
   def nh   \<equiv> "fst nogh"
   def trh  \<equiv> "snd nogh"
   def th   \<equiv> "fst trh"
@@ -243,7 +268,7 @@ lemma mwov_empty:
     shows "v = []" using assms
 proof (induct v)
   case (Cons a v)
-  then show ?case by (case_tac "snd (lookup (norms_of_grammar gr) a)") auto
+  then show ?case by (case_tac "snd (lookup (norms_of_grammar_new gr) a)") auto
 qed auto
 
 lemma mwov_length_singleton:
@@ -283,8 +308,16 @@ lemma mwov_hd_from_nog:
       and "(vh, rules) \<in> set gr"
       and "set vt \<subseteq> keys gr"
       and "th # tt = minimal_word_of_variables gr (vh # vt)"
-    shows "th = fst (snd (lookup (norms_of_grammar gr) vh))" using assms
-by (case_tac "snd (lookup (norms_of_grammar gr) vh)") auto
+    shows "th = fst (snd (lookup (norms_of_grammar_new gr) vh))" using assms
+by (case_tac "snd (lookup (norms_of_grammar_new gr) vh)") auto
+
+lemma mwov_hd_from_nog_new:
+  assumes "gram_valid gr"
+      and "(vh, rules) \<in> set gr"
+      and "set vt \<subseteq> keys gr"
+      and "th # tt = minimal_word_of_variables gr (vh # vt)"
+    shows "th = fst (snd (lookup (norms_of_grammar_new gr) vh))" using assms
+sorry
 
 lemma mwov_prefix:
   assumes G: "gram_valid gr"
@@ -294,15 +327,15 @@ lemma mwov_prefix:
     shows "tt = minimal_word_of_variables gr ((lookup rules th) @ vt)"
 proof -
   def rth  \<equiv> "lookup rules th"
-  def nvh  \<equiv> "snd (lookup (norms_of_grammar gr) vh)"
+  def nvh  \<equiv> "snd (lookup (norms_of_grammar_new gr) vh)"
   def nth  \<equiv> "fst nvh"
   def nrth \<equiv> "snd nvh"
 
   have "th = nth" using assms by (auto simp add: nth_def nvh_def mwov_hd_from_nog)
-  then have SL: "snd (lookup (norms_of_grammar gr) vh) = (th, nrth)"
+  then have SL: "snd (lookup (norms_of_grammar_new gr) vh) = (th, nrth)"
     using nvh_def nrth_def nth_def by auto
 
-  have TN: "(th, nrth) \<in> set rules" using nog_in_rules[OF G V] SL by simp
+  have TN: "(th, nrth) \<in> set rules" using nog_new_in_rules[OF G V] SL by simp
   have LO: "lookup rules th = nrth" using lookup_from_existence gram_rules_alist[OF G V] TN .
 
   have "is_alist rules" using gram_rules_alist G V .
@@ -376,17 +409,17 @@ proof (induct gr "(minimal_word_of_variables gr v)" v rule: eat_word_induct)
 
   def rules \<equiv> "lookup gr vh"
   def   rth \<equiv> "lookup rules th"
-  def  nrth \<equiv> "snd (snd (lookup (norms_of_grammar gr) vh))"
+  def  nrth \<equiv> "snd (snd (lookup (norms_of_grammar_new gr) vh))"
 
   have VT: "set vt \<subseteq> keys gr" using normal(4) by simp
   have VR: "(vh, rules) \<in> set gr" using gram_alist[OF normal(3)] normal rules_def
     by (simp add: existence_from_lookup)
   have RA: "is_alist rules" using gram_rules_alist normal(3) VR .
 
-  have "th = fst (snd (lookup (norms_of_grammar gr) vh))"
+  have "th = fst (snd (lookup (norms_of_grammar_new gr) vh))"
     using mwov_hd_from_nog normal(3) VR VT normal(2) .
-  then have TN: "(th, nrth) = snd (lookup (norms_of_grammar gr) vh)" using nrth_def by simp
-  have TH: "th \<in> keys rules" using nog_in_rules [OF normal(3) VR] sym[OF TN] by simp
+  then have TN: "(th, nrth) = snd (lookup (norms_of_grammar_new gr) vh)" using nrth_def by simp
+  have TH: "th \<in> keys rules" using nog_new_in_rules [OF normal(3) VR] sym[OF TN] by simp
 
   have TT: "tt = minimal_word_of_variables gr (rth @ vt)" unfolding rth_def
     using mwov_prefix normal(3) VR VT normal(2) .
