Isabelle/Tests.thy
@@ -15,12 +15,11 @@ definition test_gr2 :: "(char, nat) grammar" where
 
 value "gram_valid test_gr"
 value "gram_max_vars test_gr"
-value "norms_of_grammar test_gr"
+value "norms_of_grammar_new test_gr"
 value "word_in_variables test_gr ''a'' [0]"
 value "minimal_word_of_variables test_gr [1]"
 
 value "gram_valid test_gr2"
-value "norms_of_grammar test_gr2"
 value "norms_of_grammar_new test_gr2"
 
 end
